more omnisemantics combinators

src/coqutil/Semantics/OmniSmallstepCombinators.v
@@ -85,6 +85,32 @@ Section Combinators.
     - intuition eauto using always_intro.
   Qed.
 
+  Lemma eventually_always_eventually P s :
+    eventually (always (eventually P)) s <-> always (eventually P) s.
+  Proof.
+    split; eauto using eventually_done.
+    induction 1; trivial.
+    apply always_intro; eauto.
+    eapply eventually_step; [eassumption|]; intros.
+    eapply hd_always; eauto.
+  Qed.
+
+  Lemma mk_always_eventually P s
+    (Establish: eventually P s)
+    (Preserve: forall s, P s -> step s (eventually P))
+    : always (eventually P) s.
+  Proof.
+    apply mk_always with (invariant := eventually P); trivial.
+    clear dependent s; intros s; specialize (Preserve s).
+    induction 1; eauto.
+  Qed.
+
+  Lemma always_weaken: forall (P Q : State -> Prop) initial,
+    always P initial ->
+    (forall final, P final -> Q final) ->
+    always Q initial.
+  Proof. inversion 1; esplit; eauto. Qed.
+
   CoInductive always' (P : State -> Prop) s : Prop := always'_step {
     hd_always' : P s; Q ; _ : step s Q; _ s' : Q s' -> always' P s' }.
 
@@ -97,3 +123,39 @@ Section Combinators.
   Lemma always_always' P s : always' P s -> always P s.
   Proof. exists (always' P); try inversion 1; eauto. Qed.
 End Combinators.
+
+Section Combinators2.
+  (* TODO: this section should not bake in [eventually] *)
+  Context [State: Type] (step: State -> (State -> Prop) -> Prop).
+  Context (step_weaken: forall s P Q, (forall x, P x -> Q x) -> step s P -> step s Q).
+
+  Definition successively (R : State -> State -> Prop) : State -> Prop :=
+    always (fun s continue => eventually step (fun s' => R s s' /\ continue s') s) (fun _ => True).
+
+  Lemma always_eventually_successively R (R_irrefl : forall x, not (R x x)) s0 :
+    successively R s0 -> always step (eventually step (fun s' => exists s, R s s')) s0.
+  Proof.
+    intros.
+    eapply always_weaken; cycle 1; intros.
+    { eapply eventually_weaken with (P:=fun s' => exists s, R s s' /\ successively R s');
+        firstorder eauto. }
+    apply mk_always_eventually; auto.
+    { apply always_unfold1, proj2 in H; cycle 1.
+      { intros. eapply eventually_weaken in H2; intuition eauto. }
+      eapply eventually_weaken in H; eauto; intuition eauto. }
+    clear s0 H; intros s' [s [HR H]].
+    { apply always_unfold1, proj2 in H; cycle 1.
+      { intros. eapply eventually_weaken in H2; intuition eauto. }
+      destruct H.
+      { edestruct R_irrefl; eapply H. }
+      eapply step_weaken; cycle 1; eauto.
+      intros. specialize (H0 x H1).
+      intros. eapply eventually_weaken in H0; intuition eauto.  }
+  Qed.
+
+  Lemma mk_successively R s (invariant : State -> Prop) :
+    invariant s ->
+    (forall s, invariant s -> eventually step (fun s' => R s s' /\ invariant s') s) ->
+    successively R s.
+  Proof. intros; eapply mk_always with (invariant:=invariant); trivial. Qed.
+End Combinators2.
